Upd

VRF/VRF.fst
@@ -13,6 +13,7 @@ open Hacl.Impl.Ed25519.ExtPoint
 
 type bytes = buffer FStar.UInt8.t
 private let uint32_t  = FStar.UInt32.t
+private let uint64_t = FStar.UInt64.t
 
 
 let max_input_len_8 = pow2 61
@@ -52,24 +53,16 @@ assume val scalarMultiplication : out: point -> p: point ->  k:buffer Hacl.UInt8
             (fun h0 -> live h0 p /\ live h0 k /\ live h0 out)
         )
         (ensures
-            (fun h0 _ h1 -> live h0 p /\ live h0 k /\ live h0 out /\ modifies_1 k h0 h1)    
+            (fun h0 _ h1 -> live h1 p /\ live h1 k /\ live h0 out /\ modifies_1 k h0 h1)    
         )
 
+assume val isPointOnCurve: p: point -> Stack bool
+    (requires (fun h0 -> live h0 p))    
+    (ensures (fun h0 _ h1 -> live h1 p))    
 
-val _ECVRF_prove:  pbuffer: point ->
-    input: bytes {length input < max_input_len_8 - 36  } ->
-    len_input : uint32_t {v len_input = length input} -> 
-    public_key: point -> 
-    private_key: buffer Hacl.UInt8.t {length private_key = 32} -> 
-    generator: point -> 
-    proof: bytes {length proof = v (n *^ 4ul) } ->
-    Stack unit 
-        (requires 
-            (fun h0 -> live h0 input /\ live h0 public_key /\ live h0 private_key /\ live h0 generator /\ live h0 proof )
-        )
-        (ensures
-            (fun h0 _ h1 -> live h0 input /\ live h0 public_key /\ live h0 private_key /\ live h0 generator /\ live h0 proof /\ modifies_1 proof h0 h1)
-        )
+assume val _ECP2OS: out: bytes -> p: point -> Stack unit 
+    (ensures(fun h0 -> live h0 out /\ live h0 p))
+    (ensures(fun h0 _ h1 -> live h1 p /\ live h1 out /\ modifies_1 out h0 h1))
 
 assume val random: random: bytes {length random = 32} ->     
     Stack unit 
@@ -80,19 +73,20 @@ assume val random: random: bytes {length random = 32} ->
             (fun h0 _ h1 -> live h0 random /\ modifies_1 random h0 h1)
         )
 
-assume val _ECVRF_hash_to_curve:hash: bytes -> 
+assume val _ECVRF_hash_to_curve:
+    output: point -> 
     input: bytes {length input < max_input_len_8 - 36} ->
     len_input : uint32_t {v len_input = length input} -> 
     public_key: point -> 
-    Stack unit 
+    Stack bool 
         (requires
-            (fun h0 -> live h0 hash /\ live h0 input /\ live h0 public_key)
+            (fun h0 -> live h0 output /\ live h0 input /\ live h0 public_key)
         )
         (ensures
-            (fun h0 _ h1 -> live h0 hash /\ live h0 input /\ live h0 public_key /\ modifies_1 hash h0 h1)
+            (fun h0 _ h1 -> live h1 output /\ live h1 input /\ live h1 public_key /\ modifies_1 output h0 h1)
         )
 
-assume val _ECVRF_hash_points: out: point -> 
+assume val _ECVRF_hash_points: out: bytes -> 
     p1: point -> 
     p2:point -> 
     p3: point ->
@@ -109,13 +103,136 @@ assume val _ECVRF_hash_points: out: point ->
             live h0 p3 /\  live h0 p4 /\  live h0 p5 /\  live h0 p6 /\ modifies_1 out h0 h1 )
         )
 
-let _ECVRF_prove gamma gk hk input len_input public_key private_key generator proof = 
-        let hash = create 0uy 32ul in 
-    l_ECVRF_hash_to_curve hash input len_input public_key; 
-    scalarMultiplication gamma hash private_key; 
-        let rbuffer = create 0uy 32ul in 
-    random rbuffer; 
+assume val pointCreate: unit -> Stack (p:point)
+        (requires 
+            (fun h0 -> true)
+        )
+        (ensures
+            (fun h0 r h1 -> true)
+        )
+(*))
+assume val testFunc : p: point -> Stack unit 
+    (requires
+        (fun h0 -> live h0 p)
+    )
+    (ensures
+        (fun h0 _ h1 -> live h1 p)
+    )
+
+val a: unit -> Stack unit
+    (requires (fun h0 -> true))
+    (ensures (fun h0 _ h1 -> true))
+
+let a () = 
+    let point = pointCreate () in 
+    testFunc point; ()
+*)
+
+
+
+assume val bytesMultiplication: out: bytes -> m1: bytes -> m2 : uint64_t -> mod: uint64_t -> Stack unit 
+    (requires (fun h0 -> live h0 out /\ live h0 m1))
+    (ensures (fun h0 _ h1 -> live h1 m1 /\ modifies_1 out h0 h1))
+
+assume val bytesInverse: out: bytes -> m: bytes -> Stack unit
+    (requires(fun h0 -> live h0 out /\ live h0 m))
+    (ensures (fun h0 _ h1 -> live h1 m /\ modifies_1 out h0 h1))    
+
+assume val bytesAddition: out: bytes -> m1: bytes -> m2: bytes -> Stack unit
+    (requires (fun h0 -> live h0 out /\ live h0 m1 /\ live h0 m2))
+    (ensures (fun h0 _ h1 -> live h1 out /\ modifies_1 out h0 h1 /\ live h1 m1 /\ live h1 m2))
+
+assume val bytesConcat: out: bytes -> m1: bytes -> m2: bytes -> Stack unit
+    (requires (fun h0 -> live h0 out /\ live h0 m1 /\ live h0 m2))
+    (ensures (fun h0 _ h1 -> live h1 out /\ live h1 m1 /\ live h1 m2 /\ modifies_1 out h0 h1))
+
+assume val bytesSplit: out: bytes -> m: bytes ->  p1: int -> p2: int -> Stack unit
+    (requires (fun h0 -> live h0 out /\ live h0 m))
+    (ensures (fun h0 _ h1 -> live h1 out /\ live h1 m /\ modifies_1 out h0 h1 ))
+
+val _ECVRF_prove: 
+    proof: bytes {length proof = v (n *^ 4ul) } ->
+    input: bytes {length input < max_input_len_8 - 36  } ->
+    len_input : uint32_t {v len_input = length input} -> 
+    public_key: point -> 
+    private_key: buffer Hacl.UInt8.t {length private_key = 32} -> 
+    generator: point -> 
+    field: uint64_t -> 
+    Stack bool 
+        (requires 
+            (fun h0 -> live h0 input /\ live h0 public_key /\ live h0 private_key /\ live h0 generator /\ live h0 proof )
+        )
+        (ensures
+            (fun h0 _ h1 -> live h0 input /\ live h0 public_key /\ 
+            live h0 private_key /\ live h0 generator /\ live h0 proof /\ modifies_1 proof h0 h1)
+        )
+
+let _ECVRF_prove proof input len_input public_key private_key generator field  = 
+    let h = pointCreate() in 
+    let hashResult = _ECVRF_hash_to_curve h input len_input public_key in 
+        if hashResult = false then false else 
+        let gamma = pointCreate () in 
+    scalarMultiplication gamma h private_key; 
+        let k = create 0uy 32ul in 
+        let gk = pointCreate() in 
+        let hk = pointCreate() in 
+    random k; 
     scalarMultiplication gk generator k;
     scalarMultiplication hk h k;
-        let hashpoint = create 0uy 32ul;
-    _ECVRF_hash_points hashpoint generator h public_key gamma gk hk;
+        let c = create 0uy 32ul in
+    _ECVRF_hash_points c generator h public_key gamma gk hk; 
+        let cqmod = create 0uy 32ul in 
+    bytesMultiplication cqmod c field field; (* smaller than field*)
+    bytesInverse cqmod cqmod;
+        let s = create 0uy 32ul in 
+    bytesAddition s k cqmod;
+        let fstsnd = create 0uy 64ul in 
+        let fst = create 0uy 32ul in 
+    _ECP2OS fst gamma;
+    bytesConcat fstsnd fst c;
+    bytesConcat proof fstsnd s; true
+
+val _ECVRF_proof2hash: out: bytes -> proof: bytes -> Stack unit
+(requires (fun h0 -> live h0 out /\ live h0 proof))
+(ensures (fun h0 _ h1 -> live h1 out /\ live h1 proof))
+
+let _ECVRF_proof2hash out proof = 
+    bytesSplit out proof 0 1
+
+assume val _ECVRF_decode_proof: gamma:  point -> c: bytes -> s : bytes -> pi: bytes -> Stack bool
+(requires (fun h0 -> live h0 gamma /\ live h0 c /\ live h0 s /\ live h0 pi))
+(ensures (fun h0 _ h1 -> live h1 gamma /\ live h1 c /\ live h1 s /\ 
+    live h1 pi /\ modifies_1 gamma h0 h1 /\ modifies_1 c h0 h1 /\ modifies_1 s h0 h1 ))
+
+
+val _ECVRF_verify: generator: point -> public_key : point -> pi: bytes -> input: bytes ->
+len_input : uint32_t {v len_input = length input} ->  Stack bool
+(requires (fun h0 -> live h0 generator /\ live h0 public_key /\ live h0 pi /\ live h0 input))
+(ensures (fun h0 _ h1 -> live h1 generator /\ live h1 public_key /\ live h1 pi /\ live h1 input))
+
+let _ECVRF_verify generator public_key pi input len_input = 
+        let gamma = pointCreate () in 
+        let c = create 0uy 32ul in  
+        let s = create 0uy 32ul in 
+    let decoded = _ECVRF_decode_proof gamma c s pi in 
+        if not(decoded)  then false 
+        else if not(isPointOnCurve gamma) then false
+        else 
+        let pkc = pointCreate() in 
+        let gs = pointCreate() in 
+    scalarMultiplication pkc public_key c;
+    scalarMultiplication gs generator s;
+        let u = pointCreate () in 
+    scalarAddition u pkc gs; 
+        let h = pointCreate () in 
+    let h_ = _ECVRF_hash_to_curve h input len_input public_key in 
+        if not(h_) then false else 
+        let gammac = pointCreate() in 
+        let hs = pointCreate() in 
+    scalarMultiplication gammac gamma c; 
+    scalarMultiplication hs h s;     
+        let v = pointCreate() in 
+    scalarAddition v gammac hs; 
+        let c_prime = create 0uy 32ul in 
+    _ECVRF_hash_points c_prime generator h public_key gamma u v;
+    (c = c_prime)
